parser/SLLPrediction_complete.v
@@ -31,19 +31,19 @@ Module SllPredictionCompleteFn (Import D : Defs.T).
 
   (* to do : it might be possible to remove some assumptions here *)
   Lemma sllPredict'_reject__llPredict'_neq_succ :
-    forall g pm hc cm ts sps sps' ca ca' rhs,
+    forall g pm cm ts sps sps' ca ca' hk hk' hc rhs,
       no_left_recursion g
+      -> production_map_correct pm g
       -> closure_map_correct g cm
       -> all_suffix_stacks_wf g sps
       -> all_stacks_stable sps
       -> exists_successful_sp g sps ts
-      -> cache_stores_target_results g pm hc cm ca
       -> overapprox sps' sps
-      -> sllPredict' g pm hc cm sps' ts ca = (PredReject, ca')
-      -> llPredict' hc sps ts <> PredSucc rhs.
+      -> sllPredict' pm cm sps' ts ca hk' hc = (PredReject, ca')
+      -> llPredict' pm sps ts hk <> PredSucc rhs.
   Proof.
-    intros g pm hpc cm ts; induction ts as [| (a, l) ts IH];
-      intros sps sps' ca ca' rhs hn hmc hw hs he hc ho hsll hll;
+    intros g pm cm ts; induction ts as [| (a, l) ts IH];
+      intros sps sps' ca ca' hk hk' hc rhs hn hp hmc hw hs he ho hsll hll;
       pose proof hll as hll'; simpl in hsll, hll.
     - injection hsll; intros heq' heq; subst.
       eapply handleFinalSubparsers_overapprox_reject in heq; eauto; tc.
@@ -56,50 +56,51 @@ Module SllPredictionCompleteFn (Import D : Defs.T).
         clear hll.
         eapply esp_llPredict'_succ__exists_target in hll'; eauto.
         destruct hll' as [sps'' [ht hll']].
-        destruct (Cache.find _ _) as [sps''' |] eqn:hf.
-        * apply hc in hf.
+        apply sllPredict'_cont_cases in hsll. 
+        destruct hsll as [[sps''' [hf hsll]] | [sps''' [ht' hsll]]].
+        * pose proof hf as hf'; apply hc in hf'.
+          destruct hf' as [hk'' ht'].
           eapply IH in hsll; eauto.
           -- eapply llTarget_preserves_suffix_stacks_wf_invar; eauto.
           -- eapply llTarget_preserves_stacks_stable_invar; eauto.
           -- eapply llTarget_preserves_successful_sp_invar; eauto.
           -- destruct hmc; eapply target_preserves_overapprox; eauto.
-        * destruct (sllTarget _ _ _ _) as [? | sps'''] eqn:ht'; tc.
-          eapply IH in hsll; eauto.
+        * eapply IH in hsll; eauto.
           -- eapply llTarget_preserves_suffix_stacks_wf_invar; eauto.
           -- eapply llTarget_preserves_stacks_stable_invar; eauto.
           -- eapply llTarget_preserves_successful_sp_invar; eauto.
-          -- eapply sllTarget_add_preserves_cache_invar; eauto.
           -- destruct hmc; eapply target_preserves_overapprox; eauto.
   Qed.
 
   (* This might belong somewhere else *)
   Lemma esp_llPredict'_succ__exists_target : 
-    forall g pm (hc : production_map_correct pm g) sps a l ts ys,
+    forall g pm sps a l ts hk ys,
       no_left_recursion g
       -> all_suffix_stacks_wf g sps
       -> all_stacks_stable sps
-      -> llPredict' hc sps ((a, l) :: ts) = PredAmbig ys
-      -> exists sps',
-          llTarget hc a sps = inr sps'
-          /\ llPredict' hc sps' ts = PredAmbig ys.
+      -> llPredict' pm sps ((a,l) :: ts) hk = PredAmbig ys
+      -> exists sps' hk',
+          llTarget pm a sps hk = inr sps'
+          /\ llPredict' pm sps' ts hk' = PredAmbig ys.
   Proof.
-    intros g pm hc sps a l ts ys hn hw hs hl; sis; dms; tc; eauto.
+    intros g pm sps a l ts hk ys hn hw hs hl; sis; dms; tc.
+    apply llPredict'_cont_cases in hl; destruct hl as [sps'' [ht hl]]; eauto.
   Qed.
 
   (* to do : it might be possible to remove some assumptions here *)
   Lemma sllPredict'_reject__llPredict'_neq_ambig :
-    forall g pm hc cm ts sps sps' ca ca' rhs,
+    forall g pm cm ts sps sps' hk hk' ca hc ca' rhs,
       no_left_recursion g
+      -> production_map_correct pm g
       -> closure_map_correct g cm
       -> all_suffix_stacks_wf g sps
       -> all_stacks_stable sps
-      -> cache_stores_target_results g pm hc cm ca
       -> overapprox sps' sps
-      -> sllPredict' g pm hc cm sps' ts ca = (PredReject, ca')
-      -> llPredict' hc sps ts <> PredAmbig rhs.
+      -> sllPredict' pm cm sps' ts ca hk' hc = (PredReject, ca')
+      -> llPredict' pm sps ts hk <> PredAmbig rhs.
   Proof.
-    intros g pm hpc cm ts; induction ts as [| (a, l) ts IH];
-      intros sps sps' ca ca' rhs hn hmc hw hs hc ho hsll hll;
+    intros g pm cm ts; induction ts as [| (a, l) ts IH];
+      intros sps sps' hk hk' ca hc ca' rhs hn hp hmc hw hs ho hsll hll;
       pose proof hll as hll'; simpl in hsll, hll.
     - injection hsll; intros heq' heq; subst.
       eapply handleFinalSubparsers_overapprox_reject in heq; eauto; tc.
@@ -109,38 +110,44 @@ Module SllPredictionCompleteFn (Import D : Defs.T).
         eapply overapprox_nil_cons_contra; eauto.
       + (* at least one SLL sp remains *)
         destruct (allPredictionsEqual sp sps) eqn:ha; tc.
-        destruct (llTarget _ _ _) as [? | sps''] eqn:ht; tc.        
+        apply llPredict'_cont_cases in hll.
+        destruct hll as [sps'' [ht hll]].
         destruct (allPredictionsEqual sp' sps') eqn:ha'; tc.
-        destruct (Cache.find _ _) as [sps''' |] eqn:hf.
-        * apply hc in hf.
+        apply sllPredict'_cont_cases in hsll.
+        destruct hsll as [[sps''' [hf hsll]] | [sps''' [ht' hsll]]].
+        * pose proof hf as hf'; apply hc in hf'.
+          destruct hf' as [hk'' ht'].
           eapply IH in hsll; eauto.
           -- eapply llTarget_preserves_suffix_stacks_wf_invar; eauto.
           -- eapply llTarget_preserves_stacks_stable_invar; eauto.
           -- destruct hmc; eapply target_preserves_overapprox; eauto.
-        * destruct (sllTarget _ _ _ _) as [? | sps'''] eqn:ht'; tc.
-          eapply IH in hsll; eauto.
+        * eapply IH in hsll; eauto.
           -- eapply llTarget_preserves_suffix_stacks_wf_invar; eauto.
           -- eapply llTarget_preserves_stacks_stable_invar; eauto.
-          -- eapply sllTarget_add_preserves_cache_invar; eauto.
           -- destruct hmc; eapply target_preserves_overapprox; eauto.
   Qed.
 
   Lemma ussr_sllPredict_neq_reject :
-    forall g pm hc cm fr o x suf frs w ca ca',
+    forall g pm cm fr o x suf frs ts ca hc ca',
       no_left_recursion g
+      -> production_map_correct pm g
       -> closure_map_correct g cm
       -> fr = SF o (NT x :: suf)
+      -> stack_pushes_from_keyset pm (fr, frs)
       -> suffix_stack_wf g (fr, frs)
-      -> cache_stores_target_results g pm hc cm ca
-      -> gamma_recognize g (NT x :: suf ++ unprocTailSyms frs) w
-      -> sllPredict g pm hc cm x w ca <> (PredReject, ca').
+      -> gamma_recognize g (NT x :: suf ++ unprocTailSyms frs) ts
+      -> sllPredict pm cm x ts ca hc <> (PredReject, ca').
   Proof.
-    intros g pm hpc cm fr o x suf frs w ca ca' hn hmc ? hw hc hg hp'; pose proof hmc as [hsou hcom]; subst.
+    intros g pm cm fr o x suf frs ts ca hc ca'
+           hn hpc hmc ? hk hw hg hp'; pose proof hmc as [hsou hcom]; subst.
     unfold sllPredict in hp'.
-    destruct (sllStartState _ _ _) as [? | sps'] eqn:hss'; tc.
-    destruct (llStartState hpc x (SF o (NT x :: suf), frs)) as [? | sps] eqn:hs; tc.
+    apply sllPredict_cases in hp'.
+    destruct hp' as [sps' [hss' hp']].
+    destruct (llStartState pm o x suf frs hk) as [? | sps] eqn:hs; tc.
     - eapply llStartState_never_returns_error; eauto.
-    - destruct (llPredict' hpc sps w) as [rhs | rhs | | e] eqn:hp.
+    - destruct (llPredict' pm sps ts
+                           (llStartState_preserves_push_invar _ _ _ _ _ _ _ hs))
+        as [rhs | rhs | | e] eqn:hp.
       + eapply sllPredict'_reject__llPredict'_neq_succ; eauto.
         * eapply llStartState_preserves_stacks_wf_invar; eauto.
         * eapply llStartState_all_stacks_stable; eauto.
@@ -161,19 +168,19 @@ Module SllPredictionCompleteFn (Import D : Defs.T).
   
   (* THE PRIZE *)
   Theorem ussr_adaptivePredict_neq_reject :
-    forall g pm hc cm fr o x suf frs w ca ca',
+    forall g pm cm fr o x suf frs ts ca hc hk ca',
       no_left_recursion g
+      -> production_map_correct pm g
       -> closure_map_correct g cm
-      -> cache_stores_target_results g pm hc cm ca
       -> fr = SF o (NT x :: suf)
       -> suffix_stack_wf g (fr, frs)
-      -> gamma_recognize g (unprocStackSyms (fr, frs)) w
-      -> adaptivePredict g pm hc cm x (fr, frs) w ca <> (PredReject, ca').
+      -> gamma_recognize g (unprocStackSyms (fr, frs)) ts
+      -> adaptivePredict pm cm o x suf frs ts ca hc hk <> (PredReject, ca').
   Proof.
-    intros g pm hpc cm fr o x suf frs w ca ca' ?
-           hn hm hc hw hr hp; subst; simpl in hr.
-    unfold adaptivePredict in hp.
-    dmeq hsll; dms; tc; inv hp.
+    intros g pm cm fr o x suf frs ts ca hc hk ca'
+           hn hp hm ? hw hr ha; subst; simpl in hr.
+    unfold adaptivePredict in ha.
+    dmeq hsll; dms; tc; inv ha.
     - eapply ussr_llPredict_neq_reject; eauto.
     - eapply ussr_sllPredict_neq_reject; eauto.
   Qed.
